examples/splay/splaybenchmark.dfy
@@ -1,0 +1,21 @@
+include "splaytree.dfy"
+
+method Main() {
+  var tree := new_tree();
+  assert is_valid_tree(tree);
+
+  var nInsertions := 1000 * 1000 * 100;
+
+  var i: uint64 := 0;
+  while i < nInsertions
+    invariant is_valid_tree(tree)
+  {
+    var v := (i * 1073741827) % nInsertions;
+    insert(tree, v);
+    assert v in tree_set(tree);
+    var c := contains(tree, v);
+    i := i + 1;
+  }
+  print i;
+}
+
